

1 Direct Differentiation

MP2 energy in spin-orbital formalism:

$$\begin{aligned} E^{(2)} &= \frac{1}{4} \sum_{ijab} \frac{\langle ab||ij \rangle \langle ij||ab \rangle}{f_{ii} + f_{jj} - f_{aa} - f_{bb}} \\ &= \frac{1}{4} \sum_{ijab} T_{ij}^{ab} \langle ij||ab \rangle \end{aligned} \quad (1)$$

in which we denote the MP2 amplitude:

$$T_{ij}^{ab} = \frac{\langle ab||ij \rangle}{\Delta_{ab}^{ij}} = \frac{\langle ab||ij \rangle}{f_{ii} + f_{jj} - f_{aa} - f_{bb}} \quad (2)$$

Directly differentiate the second-order energy w.r.t. perturbation parameter λ :

$$\begin{aligned} \frac{\partial E^{(2)}}{\partial \lambda} &= \frac{1}{4} \sum_{ijab} \frac{\partial}{\partial \lambda} (T_{ij}^{ab} \langle ij||ab \rangle) \\ &= \frac{1}{4} \sum_{ijab} \left(\frac{\partial T_{ij}^{ab}}{\partial \lambda} \right) \langle ij||ab \rangle + \frac{1}{4} \sum_{ijab} T_{ij}^{ab} \left(\frac{\partial \langle ij||ab \rangle}{\partial \lambda} \right) \end{aligned} \quad (3)$$

in which:

$$\frac{\partial \langle ij||ab \rangle}{\partial \lambda} = \langle i^\lambda j||ab \rangle + \langle ij^\lambda||ab \rangle + \langle ij||a^\lambda b \rangle + \langle ij||ab^\lambda \rangle \quad (4)$$

exploiting the permutational symmetry and equivalence of the dummy indices:

$$\sum_{ijab} \langle i^\lambda j||ab \rangle = \sum_{ijab} \langle j^\lambda i||ba \rangle = \sum_{jiba} \langle i^\lambda j||ab \rangle \quad (5)$$

Therefore:

$$\sum_{ijab} \langle ij||ab \rangle^\lambda = 2 \sum_{ijab} (\langle i^\lambda j||ab \rangle + \langle ij||a^\lambda b \rangle) \quad (6)$$

Then:

$$\begin{aligned} \frac{\partial T_{ij}^{ab}}{\partial \lambda} &= \frac{\partial}{\partial \lambda} \left(\frac{\langle ab||ij \rangle}{\Delta_{ab}^{ij}} \right) \\ &= \frac{\langle ab||ij \rangle^\lambda}{\Delta_{ab}^{ij}} - \frac{\langle ab||ij \rangle}{(\Delta_{ab}^{ij})^2} \left(\frac{\partial \Delta_{ab}^{ij}}{\partial \lambda} \right) \\ &= \frac{\langle ab||ij \rangle^\lambda}{\Delta_{ab}^{ij}} - \frac{\langle ab||ij \rangle}{(\Delta_{ab}^{ij})^2} (\varepsilon_i^\lambda + \varepsilon_j^\lambda - \varepsilon_a^\lambda - \varepsilon_b^\lambda) \end{aligned} \quad (7)$$

Putting eqns (6) and (7) together:

$$\begin{aligned} \frac{\partial E^{(2)}}{\partial \lambda} &= \frac{1}{4} \sum_{ijab} \langle ij||ab \rangle (T_{ij}^{ab})^\lambda + \frac{1}{4} \sum_{ijab} T_{ij}^{ab} \langle ij||ab \rangle^\lambda \\ &= \frac{1}{4} \sum_{ijab} \langle ij||ab \rangle \left(\frac{\langle ab||ij \rangle^\lambda}{\Delta_{ab}^{ij}} - \frac{\langle ab||ij \rangle}{(\Delta_{ab}^{ij})^2} (\varepsilon_i^\lambda + \varepsilon_j^\lambda - \varepsilon_a^\lambda - \varepsilon_b^\lambda) \right) + \frac{1}{4} \sum_{ijab} \langle ij||ab \rangle^\lambda T_{ij}^{ab} \\ &= \frac{1}{4} \sum_{ijab} \frac{\langle ij||ab \rangle \langle ab||ij \rangle^\lambda}{\Delta_{ab}^{ij}} + \frac{1}{4} \sum_{ijab} \frac{\langle ij||ab \rangle^\lambda \langle ab||ij \rangle}{\Delta_{ab}^{ij}} - \frac{1}{4} \sum_{ijab} \frac{\langle ij||ab \rangle \langle ab||ij \rangle}{(\Delta_{ab}^{ij})^2} (2\varepsilon_i^\lambda - 2\varepsilon_a^\lambda) \end{aligned}$$

$$\begin{aligned}
&= \frac{1}{2} \sum_{ijab} (T_{ij}^{ab})^* \langle a^\lambda b || ij \rangle + \frac{1}{2} \sum_{ijab} (T_{ij}^{ab})^* \langle ab || i^\lambda j \rangle + \frac{1}{2} \sum_{ijab} T_{ij}^{ab} \langle i^\lambda j || ab \rangle + \frac{1}{2} \sum_{ijab} T_{ij}^{ab} \langle ij || a^\lambda b \rangle \\
&\quad - \frac{1}{2} \sum_{ijab} T_{ij}^{ab} (T_{ij}^{ab})^* (\varepsilon_i^\lambda - \varepsilon_a^\lambda)
\end{aligned} \tag{8}$$

Using the expression for $|i^\lambda\rangle$ and $|a^\lambda\rangle$:

$$\begin{aligned}
\frac{\partial E^{(2)}}{\partial \lambda} &= \frac{1}{2} \sum_{ijab} (T_{ij}^{ab})^* \left(\sum_k (U_{ka}^\lambda)^* \langle kb || ij \rangle + \sum_{f \neq a} (U_{fa}^\lambda)^* \langle fb || ij \rangle + \sum_\mu C_{\mu a}^* \langle \mu^\lambda b || ij \rangle \right) \\
&\quad + \frac{1}{2} \sum_{ijab} (T_{ij}^{ab})^* \left(\sum_{k \neq i} U_{ki}^\lambda \langle ab || kj \rangle + \sum_f U_{fi}^\lambda \langle ab || fj \rangle + \sum_\mu C_{\mu i} \langle ab || \mu^\lambda j \rangle \right) \\
&\quad + \frac{1}{2} \sum_{ijab} T_{ij}^{ab} \left(\sum_{k \neq i} (U_{ki}^\lambda)^* \langle kj || ab \rangle + \sum_f (U_{fi}^\lambda)^* \langle fj || ab \rangle + \sum_\mu C_{\mu i}^* \langle \mu^\lambda j || ab \rangle \right) \\
&\quad + \frac{1}{2} \sum_{ijab} T_{ij}^{ab} \left(\sum_k U_{ka}^\lambda \langle ij || kb \rangle + \sum_{f \neq a} U_{fa}^\lambda \langle ij || fb \rangle + \sum_\mu C_{\mu a} \langle ij || \mu^\lambda b \rangle \right) \\
&\quad - \frac{1}{2} \sum_{ijab} T_{ij}^{ab} (T_{ij}^{ab})^* (\varepsilon_i^\lambda - \varepsilon_a^\lambda)
\end{aligned} \tag{9}$$

Using the orthonormality condition on $(U_{ka}^\lambda)^*$, $(U_{fa}^\lambda)^*$, $(U_{ki}^\lambda)^*$ and U_{ka}^λ , and omitting the AO terms (terms involving $|\phi_\mu\rangle$) for now:

$$\begin{aligned}
\frac{\partial E^{(2)}}{\partial \lambda} &= \frac{1}{2} \sum_{ijab} \sum_k (T_{ij}^{ab})^* \langle kb || ij \rangle (-S_{ak}^\lambda - U_{ak}^\lambda) + \frac{1}{2} \sum_{ijab} \sum_{f \neq a} (T_{ij}^{ab})^* \langle fb || ij \rangle (-S_{af}^\lambda - U_{af}^\lambda) \\
&\quad + \frac{1}{2} \sum_{ijab} \sum_{k \neq i} (T_{ij}^{ab})^* \langle ab || kj \rangle U_{ki}^\lambda + \frac{1}{2} \sum_{ijab} \sum_f (T_{ij}^{ab})^* \langle ab || fi \rangle U_{fi}^\lambda \\
&\quad + \frac{1}{2} \sum_{ijab} \sum_{k \neq i} T_{ij}^{ab} \langle kj || ab \rangle (-S_{ik}^\lambda - U_{ik}^\lambda) + \frac{1}{2} \sum_{ijab} \sum_f T_{ij}^{ab} \langle fj || ab \rangle (U_{fi}^\lambda)^* \\
&\quad + \frac{1}{2} \sum_{ijab} \sum_k T_{ij}^{ab} \langle ij || kb \rangle (-S_{ak}^\lambda - (U_{ak}^\lambda)^*) + \frac{1}{2} \sum_{ijab} \sum_{f \neq a} T_{ij}^{ab} \langle ij || fb \rangle U_{fa}^\lambda \\
&\quad - \frac{1}{2} \sum_{ijab} T_{ij}^{ab} (T_{ij}^{ab})^* (\varepsilon_i^\lambda - \varepsilon_a^\lambda) + \text{AO terms}
\end{aligned} \tag{10}$$

collecting the U_{af}^λ and U_{fa}^λ terms and swapping some dummy indices:

$$\begin{aligned}
A &= -\frac{1}{2} \sum_{ijab} \sum_{f \neq a} (T_{ij}^{ab})^* \langle fb || ij \rangle U_{af}^\lambda + \frac{1}{2} \sum_{ijab} \sum_{f \neq a} T_{ij}^{ab} \langle ij || fb \rangle U_{fa}^\lambda \\
&= -\frac{1}{2} \sum_{ijfb} \sum_{a \neq f} (T_{ij}^{fb})^* \langle ab || ij \rangle U_{fa}^\lambda + \frac{1}{2} \sum_{ijab} \sum_{f \neq a} T_{ij}^{ab} \langle ij || fb \rangle U_{fa}^\lambda \\
&= \frac{1}{2} \sum_{ijab} \sum_{f \neq a} \langle ij || fb \rangle \langle ab || ij \rangle U_{fa}^\lambda \left(\frac{1}{\Delta_{ab}^{ij}} - \frac{1}{\Delta_{fb}^{ij}} \right) \\
&= \frac{1}{2} \sum_{ijab} \sum_{f \neq a} \langle ij || fb \rangle \langle ab || ij \rangle U_{fa}^\lambda \frac{\epsilon_a - \epsilon_f}{\Delta_{ab}^{ij} \Delta_{fb}^{ij}}
\end{aligned} \tag{11}$$

using the expression for U_{fa}^λ :

$$A = \frac{1}{2} \sum_{ijab} \sum_{f \neq a} \frac{\langle ij || fb \rangle \langle ab || ij \rangle (Q_{fa}^\lambda + \sum_{gm} [U_{gm}^\lambda \langle fm || ag \rangle + (U_{gm}^\lambda)^* \langle fg || am \rangle])}{\Delta_{ab}^{ij} \Delta_{fb}^{ij}}$$

$$= \frac{1}{2} \sum_{ijab} \sum_{f \neq a} T_{ij}^{ab} (T_{ij}^{fb})^* \left(Q_{fa}^\lambda + \sum_{gm} [U_{gm}^\lambda \langle fm || ag \rangle + (U_{gm}^\lambda)^* \langle fg || am \rangle] \right) \quad (12)$$

evaluating the ε_a^λ term in $\frac{\partial E^{(2)}}{\partial \lambda}$ expression:

$$\begin{aligned} \frac{1}{2} \sum_{ijab} T_{ij}^{ab} (T_{ij}^{ab})^* \varepsilon_a^\lambda &= \frac{1}{2} \sum_{ijab} T_{ij}^{ab} (T_{ij}^{ab})^* \left(Q_{aa}^\lambda + \sum_{gm} [U_{gm}^\lambda \langle am || ag \rangle + (U_{gm}^\lambda)^* \langle ag || am \rangle] \right) \\ &= \frac{1}{2} \sum_{ijab} \sum_{f=a} T_{ij}^{ab} (T_{ij}^{fb})^* \left(Q_{fa}^\lambda + \sum_{gm} [U_{gm}^\lambda \langle fm || ag \rangle + (U_{gm}^\lambda)^* \langle fg || am \rangle] \right) \end{aligned} \quad (13)$$

add this term into A :

$$A + \frac{1}{2} \sum_{ijab} T_{ij}^{ab} (T_{ij}^{ab})^* \varepsilon_a^\lambda = \frac{1}{2} \sum_{ijabf} T_{ij}^{ab} (T_{ij}^{fb})^* \left(Q_{fa}^\lambda + \sum_{gm} [U_{gm}^\lambda \langle fm || ag \rangle + (U_{gm}^\lambda)^* \langle fg || am \rangle] \right) \quad (14)$$

Similarly, collecting the U_{ki}^λ and U_{ik}^λ terms, and add the ε_i^λ term into them we get:

$$- \frac{1}{2} \sum_{ijabk} (T_{ij}^{ab})^* T_{kj}^{ab} \left(Q_{ki}^\lambda + \sum_{gm} [U_{gm}^\lambda \langle km || ig \rangle + (U_{gm}^\lambda)^* \langle kg || im \rangle] \right) \quad (15)$$

Now looking at the S_{ak}^λ terms:

$$\begin{aligned} &- \frac{1}{2} \sum_{ijab} \sum_k (T_{ij}^{ab})^* \langle kb || ij \rangle S_{ak}^\lambda - \frac{1}{2} \sum_{ijab} \sum_k T_{ij}^{ab} \langle ij || kb \rangle S_{ak}^\lambda \\ &= - \frac{1}{2} \sum_{ijkab} S_{ak}^\lambda \left(\frac{\langle ij || ab \rangle \langle kb || ij \rangle + \langle ab || ij \rangle \langle ij || kb \rangle}{\Delta_{ab}^{ij}} \right) \end{aligned} \quad (16)$$

no further simplification for general (complex) orbitals, but could be further simplified if assumed real orbitals

Now putting these all back into eqn (10):

$$\begin{aligned} \frac{\partial E^{(2)}}{\partial \lambda} &= - \frac{1}{2} \sum_{ijkab} S_{ak}^\lambda \left(T_{ij}^{ab} \langle ij || kb \rangle + (T_{ij}^{ab})^* \langle kb || ij \rangle \right) \\ &- \frac{1}{2} \sum_{ijab} \sum_{f \neq a} (T_{ij}^{ab})^* \langle fb || ij \rangle S_{af}^\lambda - \frac{1}{2} \sum_{ijab} \sum_{k \neq i} T_{ij}^{ab} \langle kj || ab \rangle S_{ik}^\lambda \\ &+ \frac{1}{2} \sum_{ijab} \sum_f (T_{ij}^{ab})^* \langle ab || fi \rangle U_{fi}^\lambda + \frac{1}{2} \sum_{ijab} \sum_f T_{ij}^{ab} \langle fj || ab \rangle (U_{fi}^\lambda)^* \\ &- \frac{1}{2} \sum_{ijab} \sum_k (T_{ij}^{ab})^* \langle kb || ij \rangle U_{ak}^\lambda - \frac{1}{2} \sum_{ijab} \sum_k T_{ij}^{ab} \langle ij || kb \rangle (U_{ak}^\lambda)^* \\ &+ \frac{1}{2} \sum_{ijabf} T_{ij}^{ab} (T_{ij}^{fb})^* \left(Q_{fa}^\lambda + \sum_{gm} [U_{gm}^\lambda \langle fm || ag \rangle + (U_{gm}^\lambda)^* \langle fg || am \rangle] \right) \\ &- \frac{1}{2} \sum_{ijabk} (T_{ij}^{ab})^* T_{kj}^{ab} \left(Q_{ki}^\lambda + \sum_{gm} [U_{gm}^\lambda \langle km || ig \rangle + (U_{gm}^\lambda)^* \langle kg || im \rangle] \right) \end{aligned} \quad (17)$$

By defining:

$$D_{ki} = - \frac{1}{2} \sum_{jab} (T_{ij}^{ab})^* T_{kj}^{ab} \quad (18)$$

$$D_{fa} = \frac{1}{2} \sum_{ijb} (T_{ij}^{fb})^* T_{ij}^{ab} \quad (19)$$

$$I_{ik} = -\frac{1}{2} \sum_{jab} T_{ij}^{ab} \langle kj || ab \rangle \quad (20)$$

$$I_{af} = -\frac{1}{2} \sum_{ijb} (T_{ij}^{ab})^* \langle fb || ij \rangle \quad (21)$$

$$I_{ak} = -\frac{1}{2} \sum_{ijb} (T_{ij}^{ab} \langle ij || kb \rangle + (T_{ij}^{ab})^* \langle kb || ij \rangle) \quad (22)$$

the derivative becomes:

$$\begin{aligned} \frac{\partial E^{(2)}}{\partial \lambda} &= \sum_{ak} S_{ak}^\lambda I_{ak} + \sum_{a \neq f} S_{af}^\lambda I_{af} + \sum_{i \neq k} S_{ik}^\lambda I_{ik} \\ &+ \sum_{af} D_{fa} Q_{fa}^\lambda + \sum_{ik} D_{ki} Q_{ki}^\lambda \\ &+ \frac{1}{2} \sum_{ijabf} (T_{ij}^{fb})^* \langle fb || ai \rangle U_{ai}^\lambda + \frac{1}{2} \sum_{ijabf} T_{ij}^{fb} \langle aj || fb \rangle (U_{ai}^\lambda)^* \\ &- \frac{1}{2} \sum_{ijkab} (T_{kj}^{ab})^* \langle ib || kj \rangle U_{ai}^\lambda - \frac{1}{2} \sum_{ijkab} T_{kj}^{ab} \langle kj || ib \rangle (U_{ai}^\lambda)^* \\ &+ \frac{1}{2} \sum_{ijmabfg} T_{mj}^{gb} (T_{mj}^{fb})^* U_{ai}^\lambda \langle fi || ga \rangle + \frac{1}{2} \sum_{ijmabfg} T_{mj}^{gb} (T_{mj}^{fb})^* (U_{ai}^\lambda)^* \langle fa || gi \rangle \\ &- \frac{1}{2} \sum_{ijkmabg} (T_{mj}^{gb})^* T_{kj}^{gb} U_{ai}^\lambda \langle ki || ma \rangle - \frac{1}{2} \sum_{ijkmabg} (T_{mj}^{gb})^* T_{kj}^{gb} (U_{ai}^\lambda)^* \langle ka || mi \rangle \\ &= \sum_{ak} S_{ak}^\lambda I_{ak} + \sum_{a \neq f} S_{af}^\lambda I_{af} + \sum_{i \neq k} S_{ik}^\lambda I_{ik} \\ &+ \sum_{af} D_{fa} Q_{fa}^\lambda + \sum_{ik} D_{ki} Q_{ki}^\lambda \\ &+ \frac{1}{2} \sum_{ijabf} (T_{ij}^{fb})^* \langle fb || ai \rangle U_{ai}^\lambda + \frac{1}{2} \sum_{ijabf} T_{ij}^{fb} \langle aj || fb \rangle (U_{ai}^\lambda)^* \\ &- \frac{1}{2} \sum_{ijkab} (T_{kj}^{ab})^* \langle ib || kj \rangle U_{ai}^\lambda - \frac{1}{2} \sum_{ijkab} T_{kj}^{ab} \langle kj || ib \rangle (U_{ai}^\lambda)^* \\ &+ \sum_{fg} \sum_{ai} D_{fg} \langle fi || ga \rangle U_{ai}^\lambda + \sum_{fg} \sum_{ai} D_{fg} \langle fa || gi \rangle (U_{ai}^\lambda)^* \\ &+ \sum_{km} \sum_{ai} D_{km} \langle ki || ma \rangle U_{ai}^\lambda + \sum_{km} \sum_{ai} D_{km} \langle ka || mi \rangle (U_{ai}^\lambda)^* \\ &= \sum_{ai} S_{ai}^\lambda I_{ai} + \sum_{a \neq b} S_a^\lambda I_{ab} + \sum_{i \neq j} S_{ij}^\lambda I_{ij} + \sum_{ab} D_{ab} Q_{ab}^\lambda + \sum_{ij} D_{ij} Q_{ij}^\lambda \\ &+ \frac{1}{2} \sum_{ai} \sum_{jbc} (T_{ij}^{bc})^* \langle bc || ai \rangle U_{ai}^\lambda + \frac{1}{2} \sum_{ai} \sum_{jbc} T_{ij}^{bc} \langle aj || bc \rangle (U_{ai}^\lambda)^* \\ &- \frac{1}{2} \sum_{ai} \sum_{jkb} (T_{kj}^{ab})^* \langle ib || kj \rangle U_{ai}^\lambda - \frac{1}{2} \sum_{ai} \sum_{jkb} T_{kj}^{ab} \langle kj || ib \rangle (U_{ai}^\lambda)^* \\ &+ \sum_{ai} \sum_{bc} D_{bc} \langle bi || ca \rangle U_{ai}^\lambda + \sum_{ai} \sum_{bc} D_{bc} \langle ba || ci \rangle (U_{ai}^\lambda)^* \end{aligned}$$

$$\begin{aligned}
& + \sum_{ai} \sum_{jk} D_{jk} \langle ji || ka \rangle U_{ai}^\lambda + \sum_{ai} \sum_{jk} D_{jk} \langle ja || ki \rangle (U_{ai}^\lambda)^* \\
& = \sum_{ai} S_{ai}^\lambda I_{ai} + \sum_{ab} S_{ab}^\lambda I_{ab} + \sum_{ij} S_{ij}^\lambda I_{ij} + \sum_{ab} D_{ab} Q_{ab}^\lambda + \sum_{ij} D_{ij} Q_{ij}^\lambda \\
& + \text{something like } \sum_{ai} X_{ai} U_{ai}^\lambda
\end{aligned} \tag{23}$$

$\sum_{a \neq b}$ and $\sum_{i \neq j}$ terms, what about the $a = b$ and $i = j$ terms?

Should I drop the complex conjugate? but still can't see how to merge $\langle bi || ca \rangle$ and $\langle ba || ci \rangle$ terms hence could not get the same X_{ai} intermediate as in the article.

2 Some Identities

From CPHF orthonormality condition:

$$U_{pq}^\lambda + (U_{qp}^\lambda)^* + S_{pq}^\lambda = 0 \quad (24)$$

Consider the spin-orbital (and using $\mathbf{C}(\lambda) = \mathbf{C}(0)\mathbf{U}(\lambda)$):

$$\begin{aligned} |a\rangle &= |\psi_a\rangle = \sum_{\mu} C_{\mu a}(\lambda) |\phi_{\mu}\rangle \\ &= \sum_{\mu} \left(\sum_q C_{\mu q}(0) U_{qa}(\lambda) \right) |\phi_{\mu}\rangle \\ &= \sum_{\mu} \left(\sum_k C_{\mu k}(0) U_{ka}(\lambda) \right) |\phi_{\mu}\rangle + \sum_{\mu} \left(\sum_{f \neq a} C_{\mu f}(0) U_{fa}(\lambda) \right) |\phi_{\mu}\rangle \end{aligned} \quad (25)$$

Question: Why not include U_{aa} into this sum?

Taking derivative w.r.t. λ :

$$\begin{aligned} |a^\lambda\rangle &= \sum_{\mu} \left(\sum_k C_{\mu k}(0) U_{ka}^\lambda \right) |\phi_{\mu}\rangle + \sum_{\mu} \left(\sum_{f \neq a} C_{\mu f}(0) U_{fa}^\lambda \right) |\phi_{\mu}\rangle \\ &\quad + \sum_{\mu} \left(\sum_k C_{\mu k}(0) U_{ka}^\lambda \right) |\phi_{\mu}^\lambda\rangle + \sum_{\mu} \left(\sum_{f \neq a} C_{\mu f}(0) U_{fa}^\lambda \right) |\phi_{\mu}^\lambda\rangle \end{aligned} \quad (26)$$

Noticing that $\mathbf{U}(0) = \mathbf{I}$ hence $\sum_{\mu} C_{\mu k}(0) |\phi_{\mu}\rangle = |\psi_k\rangle$:

$$\begin{aligned} |a^\lambda\rangle &= \sum_k U_{ka}^\lambda |\psi_k\rangle + \sum_{f \neq a} U_{fa}^\lambda |\psi_f\rangle + \sum_{\mu q} C_{\mu q}(0) U_{qa} |\phi_{\mu}^\lambda\rangle \\ &= \sum_k U_{ka}^\lambda |k\rangle + \sum_{f \neq a} U_{fa}^\lambda |f\rangle + \sum_{\mu} C_{\mu a} |\mu^\lambda\rangle \end{aligned} \quad (27)$$

Similarly:

$$|i^\lambda\rangle = \sum_{k \neq i} U_{ki}^\lambda |k\rangle + \sum_f U_{fi}^\lambda |f\rangle + \sum_{\mu} C_{\mu i} |\mu^\lambda\rangle \quad (28)$$

Expression for CPHF coefficients (c.f. Pople et al. 1979):

$$U_{fa}^\lambda = \frac{1}{\varepsilon_a - \varepsilon_f} (Q_{fa}^\lambda + \sum_{gm} [U_{gm}^\lambda \langle fm || ag \rangle + (U_{gm}^\lambda)^* \langle fg || am \rangle]) \quad (29)$$

$$U_{ki}^\lambda = \frac{1}{\varepsilon_i - \varepsilon_k} (Q_{ki}^\lambda + \sum_{gm} [U_{gm}^\lambda \langle fm || ag \rangle + (U_{gm}^\lambda)^* \langle kg || im \rangle]) \quad (30)$$

$$\varepsilon_a^\lambda = Q_{aa}^\lambda + \sum_{gm} [U_{gm}^\lambda \langle am || ag \rangle + (U_{gm}^\lambda)^* \langle ag || am \rangle] \quad (31)$$

$$\varepsilon_i^\lambda = Q_{ii}^\lambda + \sum_{gm} [U_{gm}^\lambda \langle im || ig \rangle + (U_{gm}^\lambda)^* \langle ig || im \rangle] \quad (32)$$